Clase5.MiniLang.fst
@@ -36,10 +36,25 @@ let rec eval (#ty:l_ty) (e : expr ty) : Tot (lift ty) (decreases e) =
 let constant_fold (#ty:l_ty) (e : expr ty) : Tot (expr ty) =
   match e with
   | EAdd (EInt m) (EInt n) -> EInt (m + n)
+  | EEq (EInt m) (EInt n) -> EBool (m = n)
+  | EIf (EBool true) thenExp _ -> thenExp
+  | EIf (EBool false) _ elseExp -> elseExp
   | _ -> e (* Completar con más casos. *)
 
+let rec bottom_up_fold (#ty:l_ty) (f : # (ty': l_ty) -> expr ty' -> expr ty') (e : expr ty): Tot (expr ty) (decreases e) =
+  match e with
+  | EAdd m n -> f (EAdd (bottom_up_fold f m) (bottom_up_fold f n))
+  | EEq m n -> f (EEq (bottom_up_fold f m) (bottom_up_fold f n))
+  | EIf c t e -> f (EIf (bottom_up_fold f c) (bottom_up_fold f t) (bottom_up_fold f e))
+  | _ -> f e
+
 (* Correctitud de la optimización de constant folding *)
-let constant_fold_ok (#ty:l_ty) (e : expr ty)
-  : Lemma (ensures eval e == eval (constant_fold e))
+let rec constant_fold_ok (#ty:l_ty) (e : expr ty)
+  : Lemma (ensures eval e == eval ((bottom_up_fold constant_fold) e)) (decreases e)
 =
-  ()
+  match e with
+  | EInt _ -> ()
+  | EBool _ -> ()
+  | EAdd m n -> constant_fold_ok m; constant_fold_ok n
+  | EEq m n -> constant_fold_ok m; constant_fold_ok n
+  | EIf c t e -> constant_fold_ok c; constant_fold_ok t; constant_fold_ok e
